more

Weidenbach_Book/CDCL_Two_Watched_Literals_Implementation.thy
@@ -78,30 +78,12 @@ begin
 
 end
 
-locale twl_state\<^sub>W_clss =
-  abs_state\<^sub>W
-    \<comment> \<open>functions for clauses: \<close>
-    get_lit mset_cls
-    get_cls mset_clss
-
-    \<comment> \<open>functions for the conflicting clause:\<close>
-    mset_ccls
-
-    \<comment> \<open>functions about the state:\<close>
-      \<comment> \<open>getter:\<close>
-    conc_trail hd_raw_conc_trail raw_clauses conc_backtrack_lvl
-    raw_conc_conflicting conc_learned_clss
-      \<comment> \<open>setter:\<close>
-    cons_conc_trail tl_conc_trail add_conc_confl_to_learned_cls conc_remove_cls
-    update_conc_backtrack_lvl
-    mark_conflicting reduce_conc_trail_to resolve_conflicting
-
-      \<comment> \<open>Some specific states:\<close>
-    conc_init_state
-    restart_state
+locale abs_state\<^sub>W_clss_twl_ops =
+  raw_clss_with_update
+    get_lit mset_cls get_cls mset_clss
+    twl_cls clss_update swap_lit exists_in_unwatched
     +
-  raw_clss_with_update get_lit mset_cls get_cls mset_clss twl_cls clss_update
-    swap_lit exists_in_unwatched
+  raw_cls mset_ccls
   for
     \<comment> \<open>Clause:\<close>
     get_lit :: "'cls \<Rightarrow> 'lit \<Rightarrow> 'v literal option" and
@@ -111,16 +93,86 @@ locale twl_state\<^sub>W_clss =
     get_cls :: "'clss \<Rightarrow> 'cls_it \<Rightarrow> 'cls option" and
     mset_clss:: "'clss \<Rightarrow> 'cls multiset" and
 
-    \<comment> \<open>Conflicting clause:\<close>
-    mset_ccls :: "'ccls \<Rightarrow> 'v clause" and
-
-    \<comment> \<open>2 watched literals conversion:\<close>
     twl_cls :: "'cls \<Rightarrow> 'v literal list twl_clause" and
     clss_update :: "'clss \<Rightarrow> 'cls_it \<Rightarrow> 'cls \<Rightarrow> 'clss" and
     swap_lit :: "'cls \<Rightarrow> 'lit \<Rightarrow> 'lit \<Rightarrow> 'cls" and
     exists_in_unwatched :: "('lit \<Rightarrow> bool) \<Rightarrow> 'cls \<Rightarrow> 'lit option" and
+
+    \<comment> \<open>Conflicting clause:\<close>
+    mset_ccls :: "'ccls \<Rightarrow> 'v clause"
+begin
+
+fun mmset_of_mlit :: "'clss \<Rightarrow> ('v, 'cls_it) ann_lit \<Rightarrow> ('v, 'v clause) ann_lit"
+  where
+"mmset_of_mlit Cs (Propagated L C) = Propagated L (mset_cls (Cs \<Down> C))" |
+"mmset_of_mlit _ (Decided L) = Decided L"
+
+lemma lit_of_mmset_of_mlit[simp]:
+  "lit_of (mmset_of_mlit Cs a) = lit_of a"
+  by (cases a) auto
+
+lemma lit_of_mmset_of_mlit_set_lit_of_l[simp]:
+  "lit_of ` mmset_of_mlit Cs ` set M' = lits_of_l M'"
+  by (induction M') auto
+
+lemma map_mmset_of_mlit_true_annots_true_cls[simp]:
+  "map (mmset_of_mlit Cs) M' \<Turnstile>as C \<longleftrightarrow> M' \<Turnstile>as C"
+  by (simp add: true_annots_true_cls lits_of_def)
+
+definition clauses_of_clss where
+"clauses_of_clss N \<equiv> image_mset mset_cls (mset_clss N)"
+
+notation cls_lit (infix "\<down>" 49)
+notation clss_cls (infix "\<Down>" 49)
+notation in_cls (infix "\<in>\<down>" 49)
+notation in_clss (infix "\<in>\<Down>" 49)
+
+lemma clauses_of_clss_met_cls:
+  "set_mset (clauses_of_clss Cs) = {mset_cls (Cs \<Down> i)|i. i \<in>\<Down> Cs}"
+  unfolding clauses_of_clss_def clss_cls_def in_clss_def
+  apply (auto dest!: in_mset_clss_exists_preimage)
+  by (metis option.sel)
+
+lemma finite_mset_cls: "finite {mset_cls (Cs \<Down> i)|i. i \<in>\<Down> Cs}"
+  unfolding clauses_of_clss_met_cls[symmetric] by auto
+
+lemma clauses_of_clss_mset_met_cls:
+  assumes "distinct_mset (clauses_of_clss Cs)"
+  shows "clauses_of_clss Cs = mset_set {mset_cls (Cs \<Down> i)|i. i \<in>\<Down> Cs}"
+  using clauses_of_clss_met_cls distinct_mset_set_mset_ident[OF assms] by force
+
+end
+
+
+locale abs_state\<^sub>W_twl_ops =
+  abs_state\<^sub>W_clss_twl_ops
+    \<comment> \<open>functions for clauses: \<close>
+    cls_lit mset_cls
+    clss_cls mset_clss
+    twl_cls clss_update swap_lit exists_in_unwatched
+
+    \<comment> \<open>functions for the conflicting clause:\<close>
+    mset_ccls
+  for
+    \<comment> \<open>Clause:\<close>
+    cls_lit :: "'cls \<Rightarrow> 'lit \<Rightarrow> 'v literal option" and
+    mset_cls :: "'cls \<Rightarrow> 'v clause" and
+
+    \<comment> \<open>Multiset of Clauses:\<close>
+    clss_cls :: "'clss \<Rightarrow> 'cls_it \<Rightarrow> 'cls option" and
+    mset_clss:: "'clss \<Rightarrow> 'cls multiset" and
+
+    twl_cls :: "'cls \<Rightarrow> 'v literal list twl_clause" and
+    clss_update :: "'clss \<Rightarrow> 'cls_it \<Rightarrow> 'cls \<Rightarrow> 'clss" and
+    swap_lit :: "'cls \<Rightarrow> 'lit \<Rightarrow> 'lit \<Rightarrow> 'cls" and
+    exists_in_unwatched :: "('lit \<Rightarrow> bool) \<Rightarrow> 'cls \<Rightarrow> 'lit option" and
+
+    \<comment> \<open>Conflicting clause:\<close>
+    mset_ccls :: "'ccls \<Rightarrow> 'v clause" +
+  fixes
     conc_trail :: "'st \<Rightarrow> ('v, 'v clause) ann_lits" and
     hd_raw_conc_trail :: "'st \<Rightarrow> ('v, 'cls_it) ann_lit" and
+    prop_queue :: "'st \<Rightarrow> ('v, 'v clause) ann_lits" and
     raw_clauses :: "'st \<Rightarrow> 'clss" and
     conc_backtrack_lvl :: "'st \<Rightarrow> nat" and
     raw_conc_conflicting :: "'st \<Rightarrow> 'ccls option" and
@@ -129,24 +181,124 @@ locale twl_state\<^sub>W_clss =
 
     cons_conc_trail :: "('v, 'cls_it) ann_lit \<Rightarrow> 'st \<Rightarrow> 'st" and
     tl_conc_trail :: "'st \<Rightarrow> 'st" and
-    add_conc_confl_to_learned_cls :: "'st \<Rightarrow> 'st" and
-    conc_remove_cls :: "'cls \<Rightarrow> 'st \<Rightarrow> 'st" and
-    update_conc_backtrack_lvl :: "nat \<Rightarrow> 'st \<Rightarrow> 'st" and
-    mark_conflicting :: "'cls_it \<Rightarrow> 'st \<Rightarrow> 'st" and
     reduce_conc_trail_to :: "('v, 'v clause) ann_lits \<Rightarrow> 'st \<Rightarrow> 'st" and
-    resolve_conflicting :: "'v literal \<Rightarrow> 'cls \<Rightarrow> 'st \<Rightarrow> 'st" and
 
-    conc_init_state :: "'clss \<Rightarrow> 'st" and
-    restart_state :: "'st \<Rightarrow> 'st" +
-  fixes 
-    prop_queue :: "'st \<Rightarrow> ('v, 'v clause) ann_lits" and
     cons_prop_queue :: "('v, 'cls_it) ann_lit \<Rightarrow> 'st \<Rightarrow> 'st" and
     hd_prop_queue_to_trail :: "'st \<Rightarrow> 'st" and
     prop_queue_to_trail :: "'st \<Rightarrow> 'st" and
 
+    add_conc_confl_to_learned_cls :: "'st \<Rightarrow> 'st" and
+    conc_remove_cls :: "'cls \<Rightarrow> 'st \<Rightarrow> 'st" and
+
+    update_conc_backtrack_lvl :: "nat \<Rightarrow> 'st \<Rightarrow> 'st" and
+
+    mark_conflicting :: "'cls_it \<Rightarrow> 'st \<Rightarrow> 'st" and
+    resolve_conflicting :: "'v literal \<Rightarrow> 'cls \<Rightarrow> 'st \<Rightarrow> 'st" and
+
     get_undecided_lit :: "'st \<Rightarrow> 'v literal option" and
     get_clause_watched_by :: "'st \<Rightarrow> 'v literal \<Rightarrow> 'cls_it list" and
-    update_clause :: "'st \<Rightarrow> 'cls_it \<Rightarrow> 'cls \<Rightarrow> 'st"
+    update_clause :: "'st \<Rightarrow> 'cls_it \<Rightarrow> 'cls \<Rightarrow> 'st" and
+
+    conc_init_state :: "'clss \<Rightarrow> 'st" and
+    restart_state :: "'st \<Rightarrow> 'st"
+begin
+
+definition full_trail :: "'st \<Rightarrow> ('v, 'v clause) ann_lits" where
+"full_trail S = prop_queue S @ conc_trail S"
+
+definition conc_clauses :: "'st \<Rightarrow> 'v clauses" where
+"conc_clauses S \<equiv> image_mset mset_cls (mset_clss (raw_clauses S))"
+
+definition conc_init_clss  :: "'st \<Rightarrow> 'v literal multiset multiset" where
+"conc_init_clss = (\<lambda>S. conc_clauses S - conc_learned_clss S)"
+
+abbreviation conc_conflicting :: "'st \<Rightarrow> 'v clause option" where
+"conc_conflicting \<equiv> \<lambda>S. map_option mset_ccls (raw_conc_conflicting S)"
+
+definition state :: "'st \<Rightarrow> 'v cdcl\<^sub>W_mset" where
+"state = (\<lambda>S. (full_trail S, conc_init_clss S, conc_learned_clss S, conc_backtrack_lvl S,
+  conc_conflicting S))"
+
+fun valid_annotation :: "'st \<Rightarrow> ('a, 'cls_it) ann_lit \<Rightarrow> bool" where
+"valid_annotation S (Propagated _ E) \<longleftrightarrow> E \<in>\<Down> (raw_clauses S)" |
+"valid_annotation S (Decided _) \<longleftrightarrow> True"
+
+end
+
+
+locale abs_state\<^sub>W_twl =
+  abs_state\<^sub>W_twl_ops
+    cls_lit mset_cls
+    clss_cls mset_clss
+    twl_cls clss_update swap_lit exists_in_unwatched
+
+    \<comment> \<open>functions for the conflicting clause:\<close>
+    mset_ccls
+
+    conc_trail hd_raw_conc_trail prop_queue raw_clauses conc_backtrack_lvl raw_conc_conflicting
+
+    conc_learned_clss
+
+    cons_conc_trail tl_conc_trail reduce_conc_trail_to
+
+    cons_prop_queue hd_prop_queue_to_trail prop_queue_to_trail
+
+    add_conc_confl_to_learned_cls conc_remove_cls
+
+    update_conc_backtrack_lvl mark_conflicting resolve_conflicting
+
+    get_undecided_lit get_clause_watched_by update_clause
+
+    conc_init_state restart_state
+
+  for
+    \<comment> \<open>Clause:\<close>
+    cls_lit :: "'cls \<Rightarrow> 'lit \<Rightarrow> 'v literal option" and
+    mset_cls :: "'cls \<Rightarrow> 'v clause" and
+
+    \<comment> \<open>Multiset of Clauses:\<close>
+    clss_cls :: "'clss \<Rightarrow> 'cls_it \<Rightarrow> 'cls option" and
+    mset_clss:: "'clss \<Rightarrow> 'cls multiset" and
+
+    twl_cls :: "'cls \<Rightarrow> 'v literal list twl_clause" and
+    clss_update :: "'clss \<Rightarrow> 'cls_it \<Rightarrow> 'cls \<Rightarrow> 'clss" and
+    swap_lit :: "'cls \<Rightarrow> 'lit \<Rightarrow> 'lit \<Rightarrow> 'cls" and
+    exists_in_unwatched :: "('lit \<Rightarrow> bool) \<Rightarrow> 'cls \<Rightarrow> 'lit option" and
+
+    \<comment> \<open>Conflicting clause:\<close>
+    mset_ccls :: "'ccls \<Rightarrow> 'v clause" and
+
+    conc_trail :: "'st \<Rightarrow> ('v, 'v clause) ann_lits" and
+    hd_raw_conc_trail :: "'st \<Rightarrow> ('v, 'cls_it) ann_lit" and
+    prop_queue :: "'st \<Rightarrow> ('v, 'v clause) ann_lits" and
+    raw_clauses :: "'st \<Rightarrow> 'clss" and
+    conc_backtrack_lvl :: "'st \<Rightarrow> nat" and
+    raw_conc_conflicting :: "'st \<Rightarrow> 'ccls option" and
+
+    conc_learned_clss :: "'st \<Rightarrow> 'v clauses" and
+
+    cons_conc_trail :: "('v, 'cls_it) ann_lit \<Rightarrow> 'st \<Rightarrow> 'st" and
+    tl_conc_trail :: "'st \<Rightarrow> 'st" and
+    reduce_conc_trail_to :: "('v, 'v clause) ann_lits \<Rightarrow> 'st \<Rightarrow> 'st" and
+
+    cons_prop_queue :: "('v, 'cls_it) ann_lit \<Rightarrow> 'st \<Rightarrow> 'st" and
+    hd_prop_queue_to_trail :: "'st \<Rightarrow> 'st" and
+    prop_queue_to_trail :: "'st \<Rightarrow> 'st" and
+
+    add_conc_confl_to_learned_cls :: "'st \<Rightarrow> 'st" and
+    conc_remove_cls :: "'cls \<Rightarrow> 'st \<Rightarrow> 'st" and
+
+    update_conc_backtrack_lvl :: "nat \<Rightarrow> 'st \<Rightarrow> 'st" and
+
+    mark_conflicting :: "'cls_it \<Rightarrow> 'st \<Rightarrow> 'st" and
+    resolve_conflicting :: "'v literal \<Rightarrow> 'cls \<Rightarrow> 'st \<Rightarrow> 'st" and
+
+    get_undecided_lit :: "'st \<Rightarrow> 'v literal option" and
+    get_clause_watched_by :: "'st \<Rightarrow> 'v literal \<Rightarrow> 'cls_it list" and
+    update_clause :: "'st \<Rightarrow> 'cls_it \<Rightarrow> 'cls \<Rightarrow> 'st" and
+
+    conc_init_state :: "'clss \<Rightarrow> 'st" and
+    restart_state :: "'st \<Rightarrow> 'st" +
   assumes
     state_cons_prop_queue:
       "undefined_lit (conc_trail T @ prop_queue T) (lit_of L) \<Longrightarrow>
@@ -155,20 +307,20 @@ locale twl_state\<^sub>W_clss =
       "undefined_lit (conc_trail T @ prop_queue T) (lit_of L) \<Longrightarrow>
          prop_queue (cons_prop_queue L T) = mmset_of_mlit (raw_clauses T) L # prop_queue T" and
     hd_prop_queue_to_trail_state:
-      "prop_queue T \<noteq> [] \<Longrightarrow> 
+      "prop_queue T \<noteq> [] \<Longrightarrow>
         state T = (M, N, U, k, C) \<Longrightarrow>
-        state (hd_prop_queue_to_trail T) = 
+        state (hd_prop_queue_to_trail T) =
            (hd (prop_queue T) # M, N, U, k, C)" and
     hd_prop_queue_to_trail:
-      "prop_queue T \<noteq> [] \<Longrightarrow> 
-        prop_queue (hd_prop_queue_to_trail T) = 
+      "prop_queue T \<noteq> [] \<Longrightarrow>
+        prop_queue (hd_prop_queue_to_trail T) =
            tl (prop_queue T)" and
     prop_queue_to_trail_state:
       "state T = (M, N, U, k, C) \<Longrightarrow>
         state (prop_queue_to_trail T) = (prop_queue (prop_queue_to_trail T) @ M, N, U, k, C)" and
     prop_queue_to_trail:
       "prop_queue (prop_queue_to_trail T) = []" and
-      
+
     get_undecided_lit_Some:
       "get_undecided_lit T = Some L' \<Longrightarrow> undefined_lit (conc_trail T) L' \<and>
         atm_of L' \<in> atms_of_mm (conc_clauses T)" and
@@ -180,7 +332,24 @@ locale twl_state\<^sub>W_clss =
     get_clause_watched_by_distinct:
       "distinct (get_clause_watched_by T K)" and
     update_clause:
-      "raw_clauses (update_clause S i E) = (raw_clauses S) (i := E)"
+      "i \<in>\<Down> raw_clauses S \<Longrightarrow>
+        clss_cls (raw_clauses (update_clause S i E)) = (clss_cls (raw_clauses S)) (i := Some E)" and
+    update_clause_state:
+      "i \<in>\<Down> raw_clauses S \<Longrightarrow> state S = (M, N, U, k, C) \<Longrightarrow>
+        state (update_clause S i E) = (M, conc_init_clss S, conc_learned_clss S, k, C)"
+begin
+
+lemma
+  assumes
+    "i \<in>\<Down> raw_clauses S"
+  shows
+    "conc_clauses (update S i E) =
+       remove1_mset (mset_cls (raw_clauses S \<Down> i)) (conc_clauses S) + {#E#}"
+    unfolding conc_clauses_def
+    apply (subst update_clause)
+    apply (simp add: update_clause assms)
+
+end
 
 locale abs_conflict_driven_clause_learning\<^sub>W_clss =
   twl_state\<^sub>W_clss
@@ -190,7 +359,7 @@ locale abs_conflict_driven_clause_learning\<^sub>W_clss =
 
     \<comment> \<open>functions for the conflicting clause:\<close>
     mset_ccls
-    
+
     twl_cls clss_update swap_lit  exists_in_unwatched
     \<comment> \<open>functions about the state:\<close>
       \<comment> \<open>getter:\<close>
@@ -204,22 +373,22 @@ locale abs_conflict_driven_clause_learning\<^sub>W_clss =
       \<comment> \<open>Some specific states:\<close>
     conc_init_state
     restart_state
-    
+
       -- \<open>Additional functions:\<close>
         -- \<open>Propagate queue\<close>
     prop_queue
-    cons_prop_queue 
-    hd_prop_queue_to_trail 
-    prop_queue_to_trail 
-    
+    cons_prop_queue
+    hd_prop_queue_to_trail
+    prop_queue_to_trail
+
         -- \<open>Not decided literals\<close>
-    get_undecided_lit 
+    get_undecided_lit
 
         -- \<open>Watched clauses:\<close>
     get_clause_watched_by
-    
+
     update_clause
-  
+
   for
     \<comment> \<open>Clause:\<close>
     cls_lit :: "'cls \<Rightarrow> 'lit \<Rightarrow> 'v literal" and
@@ -283,12 +452,12 @@ fun update_clause where
      if L' \<in> lits_of_l (conc_trail S)
      then S
      else
-       (case exists_in_unwatched 
+       (case exists_in_unwatched
          (\<lambda>j. undefined_lit (conc_trail S) ((raw_clauses S \<Down> i) \<down> j)) (raw_clauses S \<Down> i) of
          None \<Rightarrow> mark_conflicting i S
        | Some _ \<Rightarrow> S)
      )"
-     
+
 end
 
 
